Cleaning up: merged Decompositions

src/Decomposition.v
@@ -1,662 +1,1118 @@
-Require Import Bool List String Structures.Equalities FunctionalExtensionality Program.Equality Eqdep Eqdep_dec.
+Require Import Bool List String.
+Require Import Structures.Equalities FunctionalExtensionality Program.Equality Eqdep Eqdep_dec.
 Require Import Lib.Struct Lib.Word Lib.CommonTactics Lib.StringBound Lib.ilist Lib.FMap.
-Require Import Syntax Semantics SemFacts Wf.
+Require Import Syntax Semantics SemFacts Wf Refinement.
 
 Set Implicit Arguments.
 
-Section Decomposition.
-  Variable imp spec: Modules.
-  Variable theta: RegsT -> RegsT.
-  Variable ruleMap: RegsT -> string -> option string.
+Section GivenLabelMap.
   Variable p: string -> (sigT SignT) -> option (sigT SignT).
-  Variable thetaInit: theta (initRegs (getRegInits imp)) = initRegs (getRegInits spec).
-  Variable defSubset: forall f, In f (getDefs spec) -> In f (getDefs imp).
-  Variable callSubset: forall f, In f (getCalls spec) -> In f (getCalls imp).
-
-  Variable substepRuleMap:
-    forall oImp uImp rule csImp,
-      reachable oImp imp ->
-      Substep imp oImp uImp (Rle (Some rule)) csImp ->
-      { uSpec |
-        Substep spec (theta oImp) uSpec (Rle (ruleMap oImp rule)) (liftToMap1 p csImp) /\
-        forall o, M.union uSpec (theta o) = theta (M.union uImp o) }.
 
   Definition liftP meth :=
     match meth with
-      | (n :: t)%struct => match p n t with
-                             | None => None
-                             | Some v => Some (n :: v)%struct
-                           end
+    | (n :: t)%struct => match p n t with
+                         | None => None
+                         | Some v => Some (n :: v)%struct
+                         end
     end.
-
-  Variable substepMethMap:
-    forall oImp uImp meth csImp,
-      reachable oImp imp ->
-      Substep imp oImp uImp (Meth (Some meth)) csImp ->
-      { uSpec |
-        Substep spec (theta oImp) uSpec (Meth (liftP meth)) (liftToMap1 p csImp) /\
-        forall o, M.union uSpec (theta o) = theta (M.union uImp o) }.
-
-  Definition ruleMapEmpty o u cs (s: Substep imp o u (Rle None) cs):
-    { uSpec |
-      Substep spec (theta o) uSpec (Rle None) (liftToMap1 p cs) /\
-      forall o', M.union uSpec (theta o') = theta (M.union u o') }.
-  Proof.
-    refine (exist _ (M.empty _) _);
-    abstract (
-        inversion s; subst; rewrite liftToMap1_empty;
-        constructor;
-        [ constructor |
-          repeat rewrite M.union_empty_L; intuition]).
-  Defined.
-
-  Definition methMapEmpty o u cs (s: Substep imp o u (Meth None) cs):
-    { uSpec |
-      Substep spec (theta o) uSpec (Meth None) (liftToMap1 p cs) /\
-      forall o', M.union uSpec (theta o') = theta (M.union u o') }.
-  Proof.
-    refine (exist _ (M.empty _) _);
-    abstract (
-        inversion s; subst; rewrite liftToMap1_empty;
-        constructor;
-        [ constructor |
-          repeat rewrite M.union_empty_L; intuition]).
-  Defined.
-
-  Definition xformUnitAnnot o rm :=
-    match rm with
-      | Rle (Some rule) => Rle (ruleMap o rule)
-      | Meth (Some meth) => Meth (liftP meth)
-      | Rle None => Rle None
-      | Meth None => Meth None
-    end.
-
-  Definition substepMap o u rm cs reachO (s: Substep imp o u rm cs) :=
-    match rm return Substep imp o u rm cs ->
-                    { uSpec |
-                      Substep spec (theta o) uSpec (xformUnitAnnot o rm) (liftToMap1 p cs) /\
-                      forall o', M.union uSpec (theta o') = theta (M.union u o') } with
-      | Rle (Some rule) => fun s => substepRuleMap reachO s
-      | Meth (Some meth) => fun s => substepMethMap reachO s
-      | Rle None => fun s => ruleMapEmpty s
-      | Meth None => fun s => methMapEmpty s
-    end s.
-
-  Definition xformSubstepRec o reachO (s': SubstepRec imp o) :=
-    match s' with
-      | {| upd := u; unitAnnot := rm; cms := cs; substep := s |} =>
-        match substepMap reachO s with
-          | exist uSpec (conj sSpec _) =>
-            {| upd := uSpec; unitAnnot := xformUnitAnnot o rm;
-               cms := liftToMap1 p cs; substep := sSpec |}
-        end
-    end.
-
-  Variable specRegsCanCombine:
-    forall o reachO (s1 s2: SubstepRec imp o) d,
-      (unitAnnot s1 = Meth (Some d) \/ unitAnnot s2 = Meth (Some d)) ->
-      M.Disj (upd s1) (upd s2) -> M.Disj (upd (xformSubstepRec reachO s1))
-                                         (upd (xformSubstepRec reachO s2)).
-
-  Lemma emptyRuleNoUpd m o u:
-    Substep m o u (Rle None) (M.empty _) ->
-    u = M.empty _.
-  Proof.
-    clear.
-    intros ss.
-    dependent induction ss; reflexivity.
-  Qed.
   
-  Lemma emptyMethNoUpd m o u:
-    Substep m o u (Meth None) (M.empty _) ->
-    u = M.empty _.
-  Proof.
-    clear.
-    intros ss.
-    dependent induction ss; reflexivity.
-  Qed.
-  
-  Lemma specRegsCanCombineAnyMeth:
-    forall o reachO (s1 s2: SubstepRec imp o) d,
-      (unitAnnot s1 = Meth d \/ unitAnnot s2 = Meth d) ->
-      M.Disj (upd s1) (upd s2) -> M.Disj (upd (xformSubstepRec reachO s1))
-                                         (upd (xformSubstepRec reachO s2)).
-  Proof.
-    intros.
-    destruct d.
-    eapply specRegsCanCombine; eauto.
-    destruct s1, s2; simpl in *.
-    destruct (substepMap reachO substep), (substepMap reachO substep0);
-      destruct a, a0; simpl in *.
-    dependent induction substep;
-    dependent induction substep0;
-    try rewrite liftToMap1_empty in *;
-    destruct H; try discriminate;
-    simpl in s, s0;
-    repeat match goal with
-             | H: Substep spec (theta o) ?P (Rle None) (M.empty _) |- _ =>
-               apply emptyRuleNoUpd in H
-             | H: Substep spec (theta o) ?P (Meth None) (M.empty _) |- _ =>
-               apply emptyMethNoUpd in H
-           end; subst; (apply M.Disj_empty_1 || apply M.Disj_empty_2).
-  Qed.
+  Section DecompositionZero.
+    Variable imp spec: Modules.
 
-  Definition specCanCombine:
-    forall o reachO (s1 s2: SubstepRec imp o),
-      canCombine s1 s2 -> canCombine (xformSubstepRec reachO s1) (xformSubstepRec reachO s2).
-  Proof.
-    intros.
-    unfold canCombine in *.
-    dest.
-    pose proof (specRegsCanCombineAnyMeth reachO _ _ H1) as useful; clear specRegsCanCombine.
-    constructor.
-    - intuition.
-    - constructor.
-      clear - H0; intros.
-      unfold xformSubstepRec in *.
-      destruct s1, s2; simpl in *.
-      destruct (substepMap reachO substep), (substepMap reachO substep0); simpl in *.
-      destruct a, a0; simpl in *.
-      unfold xformUnitAnnot in *.
-      destruct unitAnnot, unitAnnot0.
-      destruct o0, o1; try discriminate.
-      destruct o0, o1; try discriminate.
-      destruct o0, o1; try discriminate.
-      destruct o0, o1; try discriminate.
-      unfold liftP in *.
-      destruct a, a0.
-      unfold not; intros.
-      destruct x, y; simpl in *.
-      rewrite <- H2 in *.
-      case_eq (p attrName attrType);
-      case_eq (p attrName0 attrType0).
-      intros.
-      rewrite H3, H4 in *.
-      subst.
-      inversion H; inversion H1; subst.
-      specialize (H0 (attrName2 :: attrType)%struct (attrName2 :: attrType0)%struct eq_refl
-                     eq_refl); simpl in *.
-      intuition.
-      intros; subst.
-      rewrite H3 in *.
-      inversion H1; discriminate.
-      intros; subst.
-      rewrite H4 in *.
-      inversion H; discriminate.
-      intros; subst.
-      rewrite H3 in *.
-      inversion H1; discriminate.
+    Section ThetaFunc.
+      Variable theta: RegsT -> RegsT.
+      Variable ruleMap: RegsT -> string -> option string.
+      Variable thetaInit: theta (initRegs (getRegInits imp)) = initRegs (getRegInits spec).
+      Variable defsImpZero: getDefsBodies imp = nil.
+      Variable defsSpecZero: getDefsBodies spec = nil.
+    
+      Variable substepRuleMap:
+        forall oImp uImp rule csImp,
+          reachable oImp imp ->
+          Substep imp oImp uImp (Rle (Some rule)) csImp ->
+          exists uSpec,
+            Substep spec (theta oImp) uSpec (Rle (ruleMap oImp rule)) (liftToMap1 p csImp) /\
+            M.union uSpec (theta oImp) = theta (M.union uImp oImp) .
 
-      + constructor.
-        clear -H1.
-        unfold xformSubstepRec.
-        destruct s1, s2; simpl in *.
-        destruct (substepMap reachO substep), (substepMap reachO substep0).
-        destruct a, a0; simpl in *.
-        unfold xformUnitAnnot.
-        destruct unitAnnot, unitAnnot0; destruct o0, o1; destruct H1; try discriminate;
-          unfold liftP; try destruct a; try destruct (p attrName attrType); eexists; eauto.
+      Definition ruleMapEmptyZero o u cs (s: Substep imp o u (Rle None) cs):
+        exists uSpec,
+          Substep spec (theta o) uSpec (Rle None) (liftToMap1 p cs) /\
+          M.union uSpec (theta o) = theta (M.union u o).
+      Proof.
+        refine (ex_intro _ (M.empty _) _);
+          abstract (
+              inversion s; subst; rewrite liftToMap1_empty;
+              constructor;
+              [ constructor |
+                repeat rewrite M.union_empty_L; intuition]).
+      Defined.
 
-        clear -H2.
-        unfold xformSubstepRec.
-        destruct s1, s2; simpl in *.
-        destruct (substepMap reachO substep), (substepMap reachO substep0).
-        destruct a, a0; simpl in *.
-        { clear - H2.
-          unfold M.Disj in *; intros.
-          specialize (H2 k).
-          destruct H2; unfold not.
-          - left; intros.
-            apply M.MapsToIn2 in H0; dest.
-            apply liftToMap1_MapsTo in H0; dest; subst.
-            apply M.MapsToIn1 in H1; intuition.
-          - right; intros.
-            apply M.MapsToIn2 in H0; dest.
-            apply liftToMap1_MapsTo in H0; dest; subst.
-            apply M.MapsToIn1 in H1; intuition.
-        }
-  Qed.
+      Definition methMapEmptyZero o u cs (s: Substep imp o u (Meth None) cs):
+        exists uSpec,
+          Substep spec (theta o) uSpec (Meth None) (liftToMap1 p cs) /\
+          M.union uSpec (theta o) = theta (M.union u o).
+      Proof.
+        refine (ex_intro _ (M.empty _) _);
+          abstract (
+              inversion s; subst; rewrite liftToMap1_empty;
+              constructor;
+              [ constructor |
+                repeat rewrite M.union_empty_L; intuition]).
+      Defined.
 
-  Theorem substepsSpecComb o reachO:
-    forall (ss: Substeps imp o), substepsComb ss ->
-                                 substepsComb (map (@xformSubstepRec o reachO) ss).
-  Proof.
-    induction ss; intros; simpl in *; constructor; intros.
-    - dependent destruction H; intuition.
-    - dependent destruction H.
-      pose proof (proj1 (in_map_iff (@xformSubstepRec o reachO) ss s') H1) as [sImp [eqS inS]].
-      specialize (H0 _ inS); subst.
-      apply specCanCombine; intuition.
-  Qed.
+      Theorem substepMethEmptyZero o u f cs (s: Substep imp o u (Meth f) cs):
+        u = M.empty _ /\ cs = M.empty _ /\ f = None.
+      Proof.
+        inversion s; eauto; exfalso.
+        rewrite defsImpZero in HIn.
+        intuition.
+      Qed.
 
-  Definition xformLabel o l :=
-    match l with
-      | {| annot := a; defs := dfs; calls := clls |} =>
-        {| annot := match a with
+      Definition substepMethMapZero o u f cs (s: Substep imp o u (Meth (Some f)) cs):
+        exists uSpec,
+          Substep spec (theta o) uSpec (Meth (liftP f)) (liftToMap1 p cs) /\
+          M.union uSpec (theta o) = theta (M.union u o).
+      Proof.
+        refine (ex_intro _ (M.empty _) _).
+        abstract (apply substepMethEmptyZero in s; dest; subst; discriminate).
+      Defined.
+
+      Definition xformUnitAnnotZero o rm :=
+        match rm with
+        | Rle (Some rule) => Rle (ruleMap o rule)
+        | Meth (Some meth) => Meth (liftP meth)
+        | Rle None => Rle None
+        | Meth None => Meth None
+        end.
+
+      Definition substepMapZero o u rm cs reachO (s: Substep imp o u rm cs) :=
+        match rm return Substep imp o u rm cs ->
+                        exists uSpec,
+                          Substep spec (theta o) uSpec (xformUnitAnnotZero o rm)
+                                  (liftToMap1 p cs) /\
+                          M.union uSpec (theta o) = theta (M.union u o) with
+        | Rle (Some rule) => fun s => substepRuleMap reachO s
+        | Meth (Some meth) => fun s => substepMethMapZero s
+        | Rle None => fun s => ruleMapEmptyZero s
+        | Meth None => fun s => methMapEmptyZero s
+        end s.
+
+      Definition xformLabelZero o l :=
+        match l with
+        | {| annot := a; defs := dfs; calls := clls |} =>
+          {| annot := match a with
                       | Some (Some r) => Some (ruleMap o r)
                       | Some None => Some None
                       | None => None
-                    end;
-           defs := liftToMap1 p dfs;
-           calls := liftToMap1 p clls |}
-    end.
+                      end;
+             defs := liftToMap1 p dfs;
+             calls := liftToMap1 p clls |}
+        end.
 
-  Lemma wellHiddenSpec o l:
-    wellHidden imp l ->
-    wellHidden spec (xformLabel o l).
-  Proof.
-    intros [dHid cHid].
-    unfold wellHidden in *.
-    unfold xformLabel; destruct l; simpl in *.
-    clear - defSubset callSubset dHid cHid.
-    pose proof (liftToMap1_DomainSubset p defs) as dH.
-    pose proof (liftToMap1_DomainSubset p calls) as cH.
-    unfold M.DomainSubset, M.KeysDisj in *.
-    constructor; unfold not; intros.
-    - specialize (dH _ H0).
-      specialize (callSubset _ H).
-      specialize (dHid _ callSubset dH).
-      intuition.
-    - specialize (cH _ H0).
-      specialize (defSubset _ H).
-      specialize (cHid _ defSubset cH).
-      intuition.
-  Qed.
-  
-  Theorem wellHiddenEq1 m l:
-    M.KeysSubset (defs l) (getDefs m) ->
-    M.KeysSubset (calls l) (getCalls m) ->
-    wellHidden m (hide l) ->
-    forall x v1 v2, M.find x (defs l) = Some v1 ->
-                    M.find x (calls l) = Some v2 ->
-                    v1 = v2.
-  Proof.
-    intros; unfold M.KeysSubset, wellHidden, M.KeysDisj in *.
-    destruct l; unfold hide; simpl in *.
-    destruct H1 as [d c].
-    destruct (signIsEq v1 v2).
-    - assumption.
-    - exfalso.
-      pose proof (M.subtractKV_in_find signIsEq H2 H3 n) as sthSub.
-      elim (d x); auto.
-      apply H0.
-      apply M.F.P.F.in_find_iff.
-      rewrite H3; discriminate.
-  Qed.
-    
-  Theorem xformLabelHideCommute o l:
-    (forall x v1 v2, M.find x (defs l) = Some v1 -> M.find x (calls l) = Some v2 -> v1 = v2) ->
-    xformLabel o (hide l) = hide (xformLabel o l).
-  Proof.
-    intros Hyp.
-    unfold xformLabel, hide.
-    destruct l as [ann ds cs]; simpl in *; f_equal.
-    - apply eq_sym, liftToMap1_subtractKV_2; auto.
-    - apply eq_sym, liftToMap1_subtractKV_2.
-      intros; apply eq_sym.
-      eapply Hyp; eauto.
-  Qed.
+      Theorem stepMapZero o (reachO: reachable o imp) u l (s: Step imp o u l):
+        exists uSpec,
+          Step spec (theta o) uSpec (xformLabelZero o l) /\
+          M.union uSpec (theta o) = theta (M.union u o).
+      Proof.
+        apply step_zero in s; auto; dest.
+        destruct l; simpl in *.
+        pose proof (substepMapZero reachO H0); dest.
+        exists x.
+        apply substepZero_imp_step in H1; auto.
+        repeat (try constructor; auto).
+        rewrite H.
+        rewrite liftToMap1_empty.
+        unfold xformUnitAnnotZero, getLabel; simpl in *.
+        destruct annot; auto.
+        destruct o0; auto.
+      Qed.
 
-  Theorem liftToMap1UnionCommute l1 l2:
-    M.Disj l1 l2 ->
-    liftToMap1 p (M.union l1 l2) = M.union (liftToMap1 p l1) (liftToMap1 p l2).
-  Proof.
-    clear; intros disj.
-    apply M.leibniz.
-    apply M.F.P.F.Equal_mapsto_iff; intros.
-    constructor; intros.
-    - apply liftToMap1_MapsTo in H; dest.
-      apply M.mapsto_union in H0.
-      apply M.mapsto_union.
-      destruct H0; dest; subst.
-      + left.
-        apply liftToMap1_MapsTo.
-        eexists; eauto.
-      + right.
-        constructor; unfold not; intros.
-        apply M.MapsToIn2 in H2; dest.
-        apply liftToMap1_MapsTo in H2; dest; subst.
-        apply M.MapsToIn1 in H3; intuition.
-        apply liftToMap1_MapsTo.
-        exists x; intuition.
-    - apply M.mapsto_union in H.
-      apply liftToMap1_MapsTo.
-      destruct H; dest; subst.
-      + apply liftToMap1_MapsTo in H; dest; subst.
-        exists x; intuition.
-        apply M.mapsto_union; intuition.
-      + apply liftToMap1_MapsTo in H0; dest; subst.
-        unfold M.Disj in disj.
-        pose proof H1 as sth.
-        apply M.MapsToIn1 in H1.
-        destruct (disj k); clear disj; intuition.
-        exists x; intuition.
-        apply M.mapsto_union; intuition.
-  Qed.
+      Lemma rleEmptyZero m o u cs:
+        Substep m o u (Rle None) cs -> u = M.empty _ /\ cs = M.empty _.
+      Proof.
+        clear;
+          intros.
+        inversion H; intuition.
+      Qed.
 
-  Theorem xformLabelAddLabelCommute l1 l2:
-    M.Disj (defs l1) (defs l2) ->
-    M.Disj (calls l1) (calls l2) ->
-    forall o,
-      xformLabel o (mergeLabel l1 l2) = mergeLabel (xformLabel o l1) (xformLabel o l2).
-  Proof.
-    intros.
-    unfold mergeLabel, xformLabel; simpl in *.
-    destruct l1, l2; simpl in *.
-    destruct annot, annot0;
-      repeat (try destruct o0; try destruct o1; simpl in *;
-              repeat rewrite liftToMap1UnionCommute; intuition).
-  Qed.
+      Lemma methEmptyZero m o u cs:
+        Substep m o u (Meth None) cs -> u = M.empty _ /\ cs = M.empty _.
+      Proof.
+        clear;
+          intros.
+        inversion H; intuition.
+      Qed.
 
-  Lemma xformLabelGetSLabelCommute o reachO a:
-    xformLabel o (getSLabel (o := o) a) = getSLabel (xformSubstepRec reachO a).
-  Proof.
-    destruct a; simpl in *.
-    destruct (substepMap reachO substep).
-    destruct a.
-    simpl.
-    unfold xformLabel, xformUnitAnnot.
-    destruct unitAnnot; destruct o0; try rewrite liftToMap1Empty; intuition.
-    destruct a.
-    unfold liftP.
-    rewrite liftToMap1_add_one.
-    unfold getSLabel; simpl.
-    destruct (p attrName attrType); intuition.
-  Qed.
-    
-  Lemma defsDisjSs' m o u n ar cms
-        (s: Substep m o u (Meth (Some (n :: ar)%struct)) cms) ss:
-    (forall s', In s' ss -> canCombine {| substep := s |} s') ->
-    M.Disj (M.add n ar (M.empty _)) (defs (foldSSLabel ss)).
-  Proof.
-    clear.
-    dependent induction ss; intros; simpl in *.
-    - apply M.Disj_empty_2.
-    - assert (sth: forall s', In s' ss ->
-                              canCombine {| substep := s |} s') by
-          (intros; specialize (H s'); intuition).
-      specialize (IHss sth); clear sth.
-      assert (sth2: canCombine {| substep := s |} a) by (specialize (H a); intuition).
-      clear H; unfold canCombine in *.
-      dest.
-      clear H x H1 H2; simpl in *.
-      destruct a.
-      unfold addLabelLeft, mergeLabel, getSLabel, getLabel; simpl in *.
-      destruct (foldSSLabel ss); simpl in *.
-      destruct unitAnnot; simpl in *.
-      + rewrite M.union_empty_L.
+      Theorem decompositionZero':
+        forall s sig, Behavior imp s sig ->
+                      exists sigSpec, Behavior spec (theta s) sigSpec /\
+                                      equivalentLabelSeq (liftToMap1 p) sig sigSpec.
+      Proof.
+        intros.
+        dependent induction H.
+        dependent induction HMultistepBeh; subst.
+        - exists nil; rewrite thetaInit; repeat constructor.
+        - specialize (IHHMultistepBeh thetaInit defsSpecZero substepRuleMap eq_refl).
+          assert(reachO: reachable n imp) by (eexists; econstructor; eauto).
+          pose proof (stepMapZero reachO HStep) as [uSpec [stepSpec upd]].
+          destruct IHHMultistepBeh as [sigSpec [behSpec eqv]].
+          inversion behSpec; subst.
+          pose proof (BehaviorIntro (Multi HMultistepBeh0 stepSpec)) as sth.
+          rewrite upd in sth.
+          exists (xformLabelZero n l :: sigSpec).
+          constructor.
+          + intuition.
+          + constructor.
+            * unfold equivalentLabel, xformLabelZero; simpl.
+              destruct l; destruct annot; simpl; intuition.
+              destruct o; simpl; intuition.
+            * intuition.
+      Qed.
+
+      Theorem decompositionZero:
+        traceRefines (liftToMap1 p) imp spec.
+      Proof.
+        unfold traceRefines; intros.
+        pose proof (decompositionZero' H) as [sigSpec beh].
+        exists (theta s1); exists sigSpec.
         intuition.
-      + destruct o0.
-        * destruct a.
-          { apply M.Disj_union.
-            - specialize (H0 (n :: ar)%struct (attrName :: attrType)%struct eq_refl eq_refl).
-              apply M.Disj_add_1.
-              apply M.Disj_empty_1.
-              unfold not; intros.
-              simpl in *.
-              apply M.F.P.F.add_in_iff in H.
-              destruct H; intuition.
-              apply M.F.P.F.empty_in_iff in H.
-              intuition.
-            - intuition.
-          } 
-        * rewrite M.union_empty_L.
-          intuition.
-  Qed.
+      Qed.
+
+    End ThetaFunc.
+    
+    Section ThetaRel.
+      Variable thetaR: RegsT -> RegsT -> Prop.
+      Variable ruleMap: RegsT -> string -> option string.
+      Variable thetaInit: thetaR (initRegs (getRegInits imp)) (initRegs (getRegInits spec)).
+      Variable defsImpZero: getDefsBodies imp = nil.
+      Variable defsSpecZero: getDefsBodies spec = nil.
+
+      Variable substepRuleMap:
+        forall oImp uImp rule csImp
+               (Hreach: reachable oImp imp),
+          Substep imp oImp uImp (Rle (Some rule)) csImp ->
+          forall oSpec,
+            thetaR oImp oSpec ->
+            exists uSpec,
+              Substep spec oSpec uSpec (Rle (ruleMap oImp rule)) (liftToMap1 p csImp) /\
+              thetaR (M.union uImp oImp) (M.union uSpec oSpec).
+
+      Definition xformLabelZeroR o l :=
+        match l with
+        | {| annot := a; defs := dfs; calls := clls |} =>
+          {| annot := match a with
+                      | Some (Some r) => Some (ruleMap o r)
+                      | Some None => Some None
+                      | None => None
+                      end;
+             defs := liftToMap1 p dfs;
+             calls := liftToMap1 p clls |}
+        end.
+
+      Lemma stepMapZeroR:
+        forall o (reachO: reachable o imp)
+               u l (s: Step imp o u l) oSpec,
+          thetaR o oSpec ->
+          exists uSpec,
+            Step spec oSpec uSpec (xformLabelZeroR o l) /\
+            thetaR (M.union u o) (M.union uSpec oSpec).
+      Proof.
+        intros; apply step_zero in s; auto; dest.
+        destruct l as [ann ds cs]; simpl in *; subst.
+
+        destruct ann as [[r|]|].
+
+        - pose proof (substepRuleMap reachO H1 H).
+          destruct H0 as [uSpec ?]; dest.
+          exists uSpec; split.
+          + apply substepZero_imp_step in H0; auto.
+          + auto.
+
+        - inv H1; exists (M.empty _); split.
+          + match goal with
+            | [ |- Step _ _ _ ?l ] =>
+              change l with (getLabel (Rle None) (M.empty _))
+            end.
+            apply substepZero_imp_step; auto.
+            constructor.
+          + mred; eauto.
+
+        - inv H1; exists (M.empty _); split.
+          + match goal with
+            | [ |- Step _ _ _ ?l ] =>
+              change l with (getLabel (Meth None) (M.empty _))
+            end.
+            apply substepZero_imp_step; auto.
+            constructor.
+          + mred; eauto.
+      Qed.
+
+      Lemma multistepMapZeroR:
+        forall o u l,
+          o = initRegs (getRegInits imp) ->
+          Multistep imp o u l ->
+          exists uSpec ll,
+            thetaR u uSpec /\
+            equivalentLabelSeq (liftToMap1 p) l ll /\
+            Multistep spec (initRegs (getRegInits spec)) uSpec ll.
+      Proof.
+        induction 2; simpl; intros; repeat subst.
+
+        - do 2 eexists; repeat split.
+          + instantiate (1:= initRegs (getRegInits spec)); auto.
+          + instantiate (1:= nil); constructor.
+          + constructor; auto.
+
+        - specialize (IHMultistep eq_refl).
+          destruct IHMultistep as [puSpec [pll ?]]; dest.
+          apply stepMapZeroR with (oSpec:= puSpec) in HStep; auto;
+            [|eexists; constructor; eauto].
+          destruct HStep as [uSpec ?]; dest.
+
+          exists (M.union uSpec puSpec), (xformLabelZeroR n l :: pll).
+          repeat split; auto.
+          + constructor; auto.
+            unfold equivalentLabel, xformLabelZero; simpl.
+            destruct l; destruct annot; simpl; intuition.
+            destruct o; simpl; intuition.
+          + constructor; auto.
+      Qed.
+
+      Theorem decompositionZeroR:
+        traceRefines (liftToMap1 p) imp spec.
+      Proof.
+        unfold traceRefines; intros.
+        inv H.
+        apply multistepMapZeroR in HMultistepBeh; auto.
+        destruct HMultistepBeh as [uSpec [ll ?]]; dest.
+        exists uSpec, ll.
+        split; auto.
+        constructor; auto.
+      Qed.
+
+    End ThetaRel.
+
+  End DecompositionZero.
+
+  Section DecompositionOne.
+    Variable imp spec: Modules.
+    
+    Section EtaFunc.
+      Hypothesis HimpEquiv: ModEquiv type typeUT imp.
+
+      Variable specRegName: string.
+      Variable eta: RegsT -> option (sigT (fullType type)).
+      Definition theta (r: RegsT): RegsT :=
+        match eta r with
+        | Some er => M.add specRegName er (M.empty _)
+        | None => M.empty _
+        end.
   
-  Lemma defsDisjSs m o (ss: list (SubstepRec m o)):
-    forall b,
-      substepsComb (b :: ss) ->
-      M.Disj (defs (getSLabel b)) (defs (foldSSLabel ss)).
+      Variable ruleMap: RegsT -> string -> option string.
+      Hypothesis HthetaInit: theta (initRegs (getRegInits imp)) = initRegs (getRegInits spec).
+
+      Hypothesis HdefSubset: forall f, In f (getDefs spec) -> In f (getDefs imp).
+      Hypothesis HcallSubset: forall f, In f (getCalls spec) -> In f (getCalls imp).
+
+      Definition ConsistentUpdate (oImp oSpec: RegsT) (uImp uSpec: UpdatesT) :=
+        (uImp = M.empty _ -> uSpec = M.empty _) /\
+        (uSpec = M.empty _ -> uImp = M.empty _) /\
+        M.union uSpec (theta oImp) = theta (M.union uImp oImp).
+
+      Hypothesis HsubstepRuleMap:
+        forall oImp uImp rule csImp,
+          reachable oImp imp ->
+          Substep imp oImp uImp (Rle (Some rule)) csImp ->
+          exists uSpec,
+            Substep spec (theta oImp) uSpec (Rle (ruleMap oImp rule)) (liftToMap1 p csImp) /\
+            ConsistentUpdate oImp (theta oImp) uImp uSpec.
+      
+      Hypothesis HsubstepMethMap:
+        forall oImp uImp meth csImp,
+          reachable oImp imp ->
+          Substep imp oImp uImp (Meth (Some meth)) csImp ->
+          exists uSpec,
+            Substep spec (theta oImp) uSpec (Meth (liftP meth)) (liftToMap1 p csImp) /\
+            ConsistentUpdate oImp (theta oImp) uImp uSpec.
+
+      Definition mapUnitLabelOne o ul :=
+        match ul with
+        | Rle (Some r) => Rle (ruleMap o r)
+        | Rle None => Rle None
+        | Meth (Some dm) => Meth (liftP dm)
+        | Meth None => Meth None
+        end.
+
+      Lemma substepMapOne:
+        forall oi ui uli csi,
+          reachable oi imp ->
+          Substep imp oi ui uli csi ->
+          exists us,
+            Substep spec (theta oi) us (mapUnitLabelOne oi uli) (liftToMap1 p csi) /\
+            ConsistentUpdate oi (theta oi) ui us.
+      Proof.
+        intros; destruct uli as [[r|]|[dm|]].
+
+        - apply HsubstepRuleMap; auto.
+        - inv H0; exists (M.empty _); split.
+          + apply EmptyRule.
+          + unfold ConsistentUpdate; repeat split; auto.
+        - apply HsubstepMethMap; auto.
+        - inv H0; exists (M.empty _); split.
+          + apply EmptyMeth.
+          + unfold ConsistentUpdate; repeat split; auto.
+      Qed.
+
+      Record SubstepRel oImp :=
+        { uImp: UpdatesT;
+          ulImp: UnitLabel;
+          csImp: MethsT;
+          HssImp: Substep imp oImp uImp ulImp csImp;
+          uSpec: UpdatesT;
+          HssSpec: Substep spec (theta oImp) uSpec
+                           (mapUnitLabelOne oImp ulImp) (liftToMap1 p csImp);
+          Hcu: ConsistentUpdate oImp (theta oImp) uImp uSpec
+        }.
+
+      Definition toSubstepRecImp {oImp} (sr: SubstepRel oImp) :=
+        {| upd := uImp sr;
+           unitAnnot := ulImp sr;
+           cms := csImp sr;
+           substep := HssImp sr
+        |}.
+
+      Definition toSubstepRecSpec {oImp} (sr: SubstepRel oImp) :=
+        {| upd := uSpec sr;
+           unitAnnot := mapUnitLabelOne oImp (ulImp sr);
+           cms := liftToMap1 p (csImp sr);
+           substep := HssSpec sr
+        |}.
+
+      Inductive SubstepRels {oImp}: list (SubstepRel oImp) -> Prop :=
+      | SubstepMapNil: SubstepRels nil
+      | SubstepMapCons:
+          forall srs sr,
+            SubstepRels srs ->
+            (forall sr', In sr' srs -> canCombine (toSubstepRecImp sr)
+                                                  (toSubstepRecImp sr')) ->
+            SubstepRels (sr :: srs).
+
+      Hypothesis HcanCombine:
+        forall oi ui1 ui2 uli1 uli2 csi1 csi2,
+          reachable oi imp ->
+          Substep imp oi ui1 uli1 csi1 ->
+          Substep imp oi ui2 uli2 csi2 ->
+          CanCombineUL ui1 ui2 (getLabel uli1 csi1) (getLabel uli2 csi2) ->
+          forall us1 us2 css1 css2,
+            Substep spec (theta oi) us1 (mapUnitLabelOne oi uli1) css1 ->
+            Substep spec (theta oi) us2 (mapUnitLabelOne oi uli2) css2 ->
+            CanCombineUL us1 us2
+                         (getLabel (mapUnitLabelOne oi uli1) css1)
+                         (getLabel (mapUnitLabelOne oi uli2) css2).
+
+      Lemma substeps_substepRels_imp:
+        forall {oImp} (Hreach: reachable oImp imp)
+               (ss: Substeps imp oImp) (Hcomb: substepsComb ss),
+        exists (srs: list (SubstepRel oImp)),
+          map toSubstepRecImp srs = ss /\ SubstepRels srs.
+      Proof.
+        induction ss; simpl; intros; [exists nil; split; auto; constructor|].
+        inv Hcomb; specialize (IHss H1).
+        destruct IHss as [psrs ?]; dest.
+        destruct a as [su sul scs Hss].
+        destruct (substepMapOne Hreach Hss) as [sus ?]; dest.
+        exists ({| HssImp := Hss; HssSpec := H3; Hcu:= H4 |} :: psrs); split.
+        - simpl; f_equal; auto.
+        - constructor; auto.
+          unfold toSubstepRecImp; simpl.
+          clear -H2 H.
+          intros; apply in_map with (f:= toSubstepRecImp) in H0.
+          rewrite H in H0; auto.
+      Qed.
+
+      Lemma substepRels_canCombine:
+        forall {oi} (Hreach: reachable oi imp)
+               (srs: list (SubstepRel oi))
+               sui suli scsi sus Hssi Hsss
+               (Hcombi : forall sr' : SubstepRel oi,
+                   In sr' srs ->
+                   canCombine {| upd := sui; unitAnnot := suli; cms := scsi; substep := Hssi |}
+                              {| upd := uImp sr'; unitAnnot := ulImp sr'; cms := csImp sr';
+                                 substep := HssImp sr' |}),
+        forall s': SubstepRec spec (theta oi),
+          In s' (map toSubstepRecSpec srs) ->
+          canCombine
+            {| upd := sus;
+               unitAnnot := mapUnitLabelOne oi suli;
+               cms := liftToMap1 p scsi;
+               substep := Hsss |} s'.
+      Proof.
+        intros.
+        apply in_map_iff in H.
+        destruct H as [nsr ?]; dest; subst.
+        specialize (Hcombi _ H0); clear H0.
+        destruct nsr as [nui nuli ncsi Hnssi nus ncss Hnsss]; simpl in *.
+        unfold toSubstepRecSpec; simpl.
+
+        apply canCombine_CanCombineUL.
+        apply canCombine_CanCombineUL in Hcombi.
+        eapply HcanCombine; eauto.
+      Qed.
+
+      Lemma substepRels_substeps_spec:
+        forall {oi} (Hreach: reachable oi imp)
+               (srs: list (SubstepRel oi)),
+          SubstepRels srs ->
+          exists (ss: Substeps spec (theta oi)),
+            map toSubstepRecSpec srs = ss /\ substepsComb ss.
+      Proof.
+        induction srs; simpl; intros; [exists nil; split; auto; constructor|].
+        inv H; specialize (IHsrs H2).
+        destruct IHsrs as [pss ?]; dest.
+        destruct a as [sui suli scsi Hssi sus Hsss].
+        exists ({| substep := Hsss |} :: pss); split.
+        - simpl; f_equal; auto.
+        - constructor; auto.
+          subst; unfold toSubstepRecImp in H3; simpl in H3.
+
+          clear -H3 Hreach HcanCombine.
+          eapply substepRels_canCombine; eauto.
+      Qed.
+
+      Lemma liftPLabel_substepRels:
+        forall {oi} (srs: list (SubstepRel oi)),
+          SubstepRels srs ->
+          liftPLabel (liftToMap1 p) ruleMap oi (foldSSLabel (map toSubstepRecImp srs)) =
+          foldSSLabel (map toSubstepRecSpec srs).
+      Proof.
+        induction srs; simpl; intros; [reflexivity|].
+        inv H. specialize (IHsrs H2).
+        rewrite <-IHsrs; clear IHsrs H2.
+        unfold addLabelLeft; rewrite liftPLabel_mergeLabel.
+        f_equal.
+        - destruct a as [ui uli csi Hssi us Hsss Hcuis].
+          unfold toSubstepRecImp, toSubstepRecSpec in *; simpl in *.
+          unfold getSLabel, getLabel; f_equal; simpl; auto.
+          + destruct uli as [[|]|[|]]; auto.
+          + unfold mapUnitLabelOne, liftP.
+            destruct uli as [[|]|[|]]; auto.
+            destruct a as [an ab]; simpl.
+            rewrite liftToMap1_add_one.
+            destruct (p an ab); auto.
+            
+        - assert (forall ss: SubstepRec imp oi,
+                     In ss (map toSubstepRecImp srs) -> canCombine (toSubstepRecImp a) ss).
+          { intros; apply in_map_iff in H; dest; subst; auto. }
+          clear H3.
+          apply canCombine_consistent_1 in H; clear -H.
+          generalize dependent (foldSSLabel (map toSubstepRecImp srs)); intros.
+          inv H; dest; clear H0.
+          repeat split; auto.
+          + destruct a; simpl in *.
+            destruct ulImp0 as [|[|]]; auto.
+            destruct a as [an ab]; simpl in *.
+            destruct (annot l); auto.
+          + destruct a; simpl in *.
+            destruct ulImp0 as [|[|]]; auto.
+      Qed.
+
+      Lemma consistentUpdate_update_spec:
+        forall (oi os: RegsT) (ui us: UpdatesT),
+          ConsistentUpdate oi os ui us ->
+          us = M.empty _ \/ exists v, us = M.add specRegName v (M.empty _).
+      Proof.
+        intros; inv H; dest.
+        remember (M.find specRegName us) as uv; destruct uv.
+
+        - right; exists s; meq.
+          assert (M.find y (M.union us (theta oi)) =
+                  M.find y (theta (M.union ui oi))) by (rewrite H1; reflexivity).
+          unfold theta in H2; destruct (eta (M.union ui oi)); findeq.
+
+        - left; meq.
+          exfalso; M.cmp y specRegName.
+          + findeq.
+          + assert (M.find y (M.union us (theta oi)) =
+                    M.find y (theta (M.union ui oi))) by (rewrite H1; reflexivity).
+            unfold theta in H2; destruct (eta (M.union ui oi)); findeq.
+      Qed.
+
+      Lemma substepRels_consistentUpdate:
+        forall oi,
+          reachable oi imp ->
+          forall (srs: list (SubstepRel oi)),
+            SubstepRels srs ->
+            ConsistentUpdate oi (theta oi) (foldSSUpds (map toSubstepRecImp srs))
+                             (foldSSUpds (map toSubstepRecSpec srs)).
+      Proof.
+        induction 2; simpl; intros;
+          [unfold ConsistentUpdate; repeat split; auto|].
+
+        pose proof (consistentUpdate_update_spec IHSubstepRels).
+        unfold ConsistentUpdate in *; dest; repeat split.
+        - intros.
+          destruct sr as [ui uli csi Hssi us Hsss [? [? ?]]]; simpl in *.
+          apply M.union_empty in H6; dest.
+          unfold toSubstepRecImp in H1; simpl in H1; subst.
+          specialize (e eq_refl); subst.
+          mred.
+        - intros.
+          destruct sr as [ui uli csi Hssi us Hsss [? [? ?]]]; simpl in *.
+          apply M.union_empty in H6; dest.
+          unfold toSubstepRecImp in H1; simpl in H1; subst.
+          specialize (e0 eq_refl); subst.
+          mred.
+        - destruct H2.
+          + rewrite H2 in *.
+            specialize (H4 eq_refl); rewrite H4 in *.
+            mred.
+            clear; destruct sr; simpl in *.
+            inv Hcu0; dest; auto.
+          + destruct sr as [ui uli csi Hssi us Hsss Hcuis]; simpl in *.
+            pose proof (consistentUpdate_update_spec Hcuis).
+            unfold toSubstepRecImp in H1; simpl in H1.
+            inv Hcuis; dest.
+            destruct H6.
+
+            * subst.
+              specialize (H8 eq_refl); subst.
+              mred.
+            * exfalso.
+              pose proof (substepRels_canCombine (sui:= ui) (Hssi:= Hssi) H srs Hsss H1).
+              apply canCombine_consistent_1 in H10.
+              dest; subst.
+              rewrite H2 in H10; clear -H10.
+              inv H10; dest; clear -H.
+              specialize (H specRegName); destruct H; findeq.
+      Qed.
+
+      Lemma substepRels_wellHidden:
+        forall o,
+          reachable o imp ->
+          forall (srs: list (SubstepRel o)),
+            SubstepRels srs ->
+            wellHidden imp (hide (foldSSLabel (map toSubstepRecImp srs))) ->
+            wellHidden spec (hide (foldSSLabel (map toSubstepRecSpec srs))).
+      Proof.
+        intros.
+        pose proof (liftPLabel_wellHidden spec ruleMap o p HdefSubset HcallSubset H1).
+        rewrite liftPLabel_hide with (imp:= imp) in H2; auto.
+        - rewrite liftPLabel_substepRels in H2; auto.
+        - unfold M.KeysSubset; apply getDefs_substeps.
+        - unfold M.KeysSubset; apply getCalls_substeps; auto.
+      Qed.
+
+      Theorem decompositionOne:
+        traceRefines (liftToMap1 p) imp spec.
+      Proof.
+        apply stepRefinement with (theta:= theta) (ruleMap:= ruleMap); auto.
+        intros.
+
+        inv H0.
+        apply substeps_substepRels_imp in HSubsteps; auto.
+        destruct HSubsteps as [srs ?]; dest.
+        pose proof (substepRels_consistentUpdate H H1).
+        pose proof (substepRels_substeps_spec H H1).
+        destruct H3 as [sss ?]; dest.
+        exists (foldSSUpds sss); split.
+
+        - rewrite liftPLabel_hide with (imp:= imp); auto.
+          + subst; rewrite liftPLabel_substepRels; auto.
+            constructor; auto.
+            apply substepRels_wellHidden; auto.
+          + unfold M.KeysSubset; apply getDefs_substeps.
+          + unfold M.KeysSubset; apply getCalls_substeps; auto.
+
+        - subst; unfold ConsistentUpdate in H2; dest; auto.
+      Qed.
+      
+    End EtaFunc.
+
+    Section EtaRel.
+      Hypothesis HimpEquiv: ModEquiv type typeUT imp.
+
+      Variable specRegName: string.
+      Variable etaR: RegsT -> option (sigT (fullType type)) -> Prop.
+
+      Definition etaRState (v: option (sigT (fullType type))) :=
+        match v with
+        | Some ev => M.add specRegName ev (M.empty _)
+        | _ => M.empty _
+        end.
+      Definition thetaR (ir sr: RegsT): Prop := exists sv, etaR ir sv /\ etaRState sv = sr.
+      
+      Variable ruleMap: RegsT -> string -> option string.
+      Hypothesis HthetaRRInit: thetaR (initRegs (getRegInits imp)) (initRegs (getRegInits spec)).
+      
+      Hypothesis HdefSubset: forall f, In f (getDefs spec) -> In f (getDefs imp).
+      Hypothesis HcallSubset: forall f, In f (getCalls spec) -> In f (getCalls imp).
+
+      Definition ConsistentUpdateR (oImp oSpec: RegsT) (uImp uSpec: UpdatesT) :=
+        (uImp = M.empty _ -> uSpec = M.empty _) /\
+        (uSpec = M.empty _ -> uImp = M.empty _) /\
+        (thetaR oImp oSpec -> thetaR (M.union uImp oImp) (M.union uSpec oSpec)).
+
+      Hypothesis HsubstepRuleRel:
+        forall oImp uImp rule csImp,
+          reachable oImp imp ->
+          Substep imp oImp uImp (Rle (Some rule)) csImp ->
+          forall oSpec,
+            thetaR oImp oSpec ->
+            exists uSpec,
+              Substep spec oSpec uSpec (Rle (ruleMap oImp rule)) (liftToMap1 p csImp) /\
+              ConsistentUpdateR oImp oSpec uImp uSpec.
+
+      Hypothesis HsubstepMethRel:
+        forall oImp uImp meth csImp,
+          reachable oImp imp ->
+          Substep imp oImp uImp (Meth (Some meth)) csImp ->
+          forall oSpec,
+            thetaR oImp oSpec ->
+            exists uSpec,
+              Substep spec oSpec uSpec (Meth (liftP meth)) (liftToMap1 p csImp) /\
+              ConsistentUpdateR oImp oSpec uImp uSpec.
+
+      Definition mapUnitLabelR o ul :=
+        match ul with
+        | Rle (Some r) => Rle (ruleMap o r)
+        | Rle None => Rle None
+        | Meth (Some dm) => Meth (liftP dm)
+        | Meth None => Meth None
+        end.
+
+      Lemma substepRel:
+        forall oi ui uli csi,
+          reachable oi imp ->
+          Substep imp oi ui uli csi ->
+          forall os,
+            thetaR oi os ->
+            exists us,
+              Substep spec os us (mapUnitLabelR oi uli) (liftToMap1 p csi) /\
+              ConsistentUpdateR oi os ui us.
+      Proof.
+        intros; destruct uli as [[r|]|[dm|]].
+
+        - apply HsubstepRuleRel; auto.
+        - inv H0; exists (M.empty _); split.
+          + apply EmptyRule.
+          + unfold ConsistentUpdate; repeat split; auto.
+        - apply HsubstepMethRel; auto.
+        - inv H0; exists (M.empty _); split.
+          + apply EmptyMeth.
+          + unfold ConsistentUpdate; repeat split; auto.
+      Qed.
+
+      Record SubstepRelR oImp oSpec :=
+        { uImpR: UpdatesT;
+          ulImpR: UnitLabel;
+          csImpR: MethsT;
+          HssImpR: Substep imp oImp uImpR ulImpR csImpR;
+          uSpecR: UpdatesT;
+          HssSpecR: Substep spec oSpec uSpecR
+                            (mapUnitLabelR oImp ulImpR) (liftToMap1 p csImpR);
+          HthetaR: thetaR oImp oSpec;
+          HcuR: ConsistentUpdateR oImp oSpec uImpR uSpecR
+        }.
+
+      Definition toSubstepRecImpR {oImp oSpec} (sr: SubstepRelR oImp oSpec) :=
+        {| upd := uImpR sr;
+           unitAnnot := ulImpR sr;
+           cms := csImpR sr;
+           substep := HssImpR sr
+        |}.
+
+      Definition toSubstepRecSpecR {oImp oSpec} (sr: SubstepRelR oImp oSpec) :=
+        {| upd := uSpecR sr;
+           unitAnnot := mapUnitLabelR oImp (ulImpR sr);
+           cms := liftToMap1 p (csImpR sr);
+           substep := HssSpecR sr
+        |}.
+
+      Inductive SubstepRelsR {oImp oSpec}: list (SubstepRelR oImp oSpec) -> Prop :=
+      | SubstepMapNilR: SubstepRelsR nil
+      | SubstepMapConsR:
+          forall srs sr,
+            SubstepRelsR srs ->
+            (forall sr', In sr' srs -> canCombine (toSubstepRecImpR sr)
+                                                  (toSubstepRecImpR sr')) ->
+            SubstepRelsR (sr :: srs).
+
+      Hypothesis HcanCombine:
+        forall oi ui1 ui2 uli1 uli2 csi1 csi2,
+          reachable oi imp ->
+          Substep imp oi ui1 uli1 csi1 ->
+          Substep imp oi ui2 uli2 csi2 ->
+          CanCombineUL ui1 ui2 (getLabel uli1 csi1) (getLabel uli2 csi2) ->
+          forall us1 us2 css1 css2 os,
+            thetaR oi os ->
+            Substep spec os us1 (mapUnitLabelR oi uli1) css1 ->
+            Substep spec os us2 (mapUnitLabelR oi uli2) css2 ->
+            CanCombineUL us1 us2
+                         (getLabel (mapUnitLabelR oi uli1) css1)
+                         (getLabel (mapUnitLabelR oi uli2) css2).
+
+      Lemma substeps_substepRels_impR:
+        forall {oImp oSpec} (HthetaR: thetaR oImp oSpec)
+               (Hreach: reachable oImp imp)
+               (ss: Substeps imp oImp) (Hcomb: substepsComb ss),
+        exists (srs: list (SubstepRelR oImp oSpec)),
+          map toSubstepRecImpR srs = ss /\ SubstepRelsR srs.
+      Proof.
+        induction ss; simpl; intros; [exists nil; split; auto; constructor|].
+        inv Hcomb; specialize (IHss H1).
+        destruct IHss as [psrs ?]; dest.
+        destruct a as [su sul scs Hss].
+        pose proof (substepRel Hreach Hss HthetaR0) as [sus ?]; dest.
+        exists ({| HthetaR:= HthetaR0; HssImpR := Hss; HssSpecR := H3; HcuR:= H4 |} :: psrs); split.
+        - simpl; f_equal; auto.
+        - constructor; auto.
+          unfold toSubstepRecImp; simpl.
+          clear -H2 H.
+          intros; apply in_map with (f:= toSubstepRecImpR) in H0.
+          rewrite H in H0; auto.
+      Qed.
+
+      Lemma substepRels_canCombineR:
+        forall {oi os} (Hreach: reachable oi imp)
+               (srs: list (SubstepRelR oi os))
+               sui suli scsi sus Hssi Hsss
+               (Hcombi : forall sr' : SubstepRelR oi os,
+                   In sr' srs ->
+                   canCombine {| upd := sui; unitAnnot := suli; cms := scsi; substep := Hssi |}
+                              {| upd := uImpR sr'; unitAnnot := ulImpR sr'; cms := csImpR sr';
+                                 substep := HssImpR sr' |}),
+        forall s': SubstepRec spec os,
+          In s' (map toSubstepRecSpecR srs) ->
+          canCombine
+            {| upd := sus;
+               unitAnnot := mapUnitLabelR oi suli;
+               cms := liftToMap1 p scsi;
+               substep := Hsss |} s'.
+      Proof.
+        intros.
+        apply in_map_iff in H.
+        destruct H as [nsr ?]; dest; subst.
+        specialize (Hcombi _ H0); clear H0.
+        destruct nsr as [nui nuli ncsi Hnssi nus ncss Hnsss]; simpl in *.
+        unfold toSubstepRecSpec; simpl.
+
+        apply canCombine_CanCombineUL.
+        apply canCombine_CanCombineUL in Hcombi.
+        eapply HcanCombine; eauto.
+      Qed.
+
+      Lemma substepRels_substeps_specR:
+        forall {oi os} (Hreach: reachable oi imp)
+               (srs: list (SubstepRelR oi os)),
+          SubstepRelsR srs ->
+          exists (ss: Substeps spec os),
+            map toSubstepRecSpecR srs = ss /\ substepsComb ss.
+      Proof.
+        induction srs; simpl; intros; [exists nil; split; auto; constructor|].
+        inv H; specialize (IHsrs H2).
+        destruct IHsrs as [pss ?]; dest.
+        destruct a as [sui suli scsi Hssi sus Hsss].
+        exists ({| substep := Hsss |} :: pss); split.
+        - simpl; f_equal; auto.
+        - constructor; auto.
+          subst; unfold toSubstepRecImp in H3; simpl in H3.
+
+          clear -H3 HthetaR0 Hreach HcanCombine.
+          eapply substepRels_canCombineR; eauto.
+      Qed.
+
+      Lemma liftPLabel_substepRelsR:
+        forall {oi os} (srs: list (SubstepRelR oi os)),
+          SubstepRelsR srs ->
+          liftPLabel (liftToMap1 p) ruleMap oi (foldSSLabel (map toSubstepRecImpR srs)) =
+          foldSSLabel (map toSubstepRecSpecR srs).
+      Proof.
+        induction srs; simpl; intros; [reflexivity|].
+        inv H. specialize (IHsrs H2).
+        rewrite <-IHsrs; clear IHsrs H2.
+        unfold addLabelLeft; rewrite liftPLabel_mergeLabel.
+        f_equal.
+        - destruct a as [ui uli csi Hssi us Hsss Hcuis].
+          unfold toSubstepRecImp, toSubstepRecSpec in *; simpl in *.
+          unfold getSLabel, getLabel; f_equal; simpl; auto.
+          + destruct uli as [[|]|[|]]; auto.
+          + unfold mapUnitLabelR, liftP.
+            destruct uli as [[|]|[|]]; auto.
+            destruct a as [an ab]; simpl.
+            rewrite liftToMap1_add_one.
+            destruct (p an ab); auto.
+            
+        - assert (forall ss: SubstepRec imp oi,
+                     In ss (map toSubstepRecImpR srs) -> canCombine (toSubstepRecImpR a) ss).
+          { intros; apply in_map_iff in H; dest; subst; auto. }
+          clear H3.
+          apply canCombine_consistent_1 in H; clear -H.
+          generalize dependent (foldSSLabel (map toSubstepRecImpR srs)); intros.
+          inv H; dest; clear H0.
+          repeat split; auto.
+          + destruct a; simpl in *.
+            destruct ulImpR0 as [|[|]]; auto.
+            destruct a as [an ab]; simpl in *.
+            destruct (annot l); auto.
+          + destruct a; simpl in *.
+            destruct ulImpR0 as [|[|]]; auto.
+      Qed.
+
+      Lemma consistentUpdate_update_specR:
+        forall (oi os: RegsT) (HthetaR: thetaR oi os)
+               (ui us: UpdatesT),
+          ConsistentUpdateR oi os ui us ->
+          us = M.empty _ \/ exists v, us = M.add specRegName v (M.empty _).
+      Proof.
+        intros; inv H; dest.
+        remember (M.find specRegName us) as uv; destruct uv.
+
+        - right; exists s; meq; exfalso.
+          unfold thetaR in H2; destruct H2 as [sv ?]; dest.
+          destruct sv.
+          + simpl in H2; apply M.Equal_val with (k:= y) in H2; mred.
+          + simpl in H2; apply M.Equal_val with (k:= y) in H2; mred.
+
+        - left; meq.
+          exfalso; M.cmp y specRegName.
+          + findeq.
+          + unfold thetaR in H2; destruct H2 as [sv ?]; dest.
+            destruct sv.
+            * simpl in H2; apply M.Equal_val with (k:= y) in H2; mred.
+            * simpl in H2; apply M.Equal_val with (k:= y) in H2; mred.
+      Qed.
+
+      Lemma substepRels_consistentUpdateR:
+        forall oi os,
+          reachable oi imp ->
+          forall (srs: list (SubstepRelR oi os)),
+            SubstepRelsR srs ->
+            ConsistentUpdateR oi os (foldSSUpds (map toSubstepRecImpR srs))
+                              (foldSSUpds (map toSubstepRecSpecR srs)).
+      Proof.
+        induction 2; simpl; intros;
+          [unfold ConsistentUpdateR; repeat split; auto|].
+
+        destruct sr as [ui uli csi Hssi us Hsss HthetaR Hcu]; simpl in *.
+        pose proof (consistentUpdate_update_specR HthetaR IHSubstepRelsR).
+        repeat split.
+        - intros; unfold ConsistentUpdateR in *; dest; simpl in *.
+          apply M.union_empty in H3; dest.
+          unfold toSubstepRecImpR in H1; simpl in H1; subst.
+          specialize (e eq_refl); subst.
+          mred.
+        - intros; unfold ConsistentUpdateR in *; dest; simpl in *.
+          apply M.union_empty in H3; dest.
+          unfold toSubstepRecImpR in H1; simpl in H1; subst.
+          specialize (e0 eq_refl); subst.
+          mred.
+        - destruct H2.
+          + rewrite H2 in *.
+            unfold ConsistentUpdateR in *; dest; simpl in *.
+            specialize (H4 eq_refl); rewrite H4 in *.
+            intros; mred; auto.
+          + pose proof (consistentUpdate_update_specR HthetaR Hcu).
+            unfold toSubstepRecImpR in H1; simpl in H1.
+            inv Hcu; dest.
+            destruct H3.
+
+            * subst.
+              specialize (H5 eq_refl); subst.
+              inv IHSubstepRelsR; dest.
+              mred.
+            * exfalso.
+              pose proof (substepRels_canCombineR (sui:= ui) (Hssi:= Hssi) H srs Hsss H1).
+              apply canCombine_consistent_1 in H7.
+              dest; subst.
+              rewrite H2 in H7; clear -H7.
+              inv H7; dest; clear -H.
+              specialize (H specRegName); destruct H; findeq.
+      Qed.
+
+      Lemma substepRels_wellHiddenR:
+        forall o s,
+          reachable o imp ->
+          forall (srs: list (SubstepRelR o s)),
+            SubstepRelsR srs ->
+            wellHidden imp (hide (foldSSLabel (map toSubstepRecImpR srs))) ->
+            wellHidden spec (hide (foldSSLabel (map toSubstepRecSpecR srs))).
+      Proof.
+        intros.
+        pose proof (liftPLabel_wellHidden spec ruleMap o p HdefSubset HcallSubset H1).
+        rewrite liftPLabel_hide with (imp:= imp) in H2; auto.
+        - rewrite liftPLabel_substepRelsR in H2; auto.
+        - unfold M.KeysSubset; apply getDefs_substeps.
+        - unfold M.KeysSubset; apply getCalls_substeps; auto.
+      Qed.
+
+      Lemma stepMapOne:
+        forall o (reachO: reachable o imp)
+               u l (s: Step imp o u l) oSpec,
+          thetaR o oSpec ->
+          exists uSpec ul,
+            Step spec oSpec uSpec ul /\
+            thetaR (M.union u o) (M.union uSpec oSpec) /\
+            equivalentLabel (liftToMap1 p) l ul.
+      Proof.
+        intros; inv s.
+        pose proof (substeps_substepRels_impR H reachO HSubsteps) as Hsrs.
+        destruct Hsrs as [srs ?]; dest; subst.
+        exists (foldSSUpds (map toSubstepRecSpecR srs)).
+        exists (hide (foldSSLabel (map toSubstepRecSpecR srs))); split; [|split].
+        - constructor; auto.
+          + pose proof (substepRels_substeps_specR reachO H1) as Hsss.
+            dest; subst; auto.
+          + apply substepRels_wellHiddenR; auto.
+        - apply substepRels_consistentUpdateR; auto.
+        - pose proof (liftPLabel_substepRelsR H1).
+          rewrite <-H0.
+          rewrite <-liftPLabel_hide with (imp:= imp); auto.
+          + generalize (hide (foldSSLabel (map toSubstepRecImpR srs))) as l; intros.
+            destruct l as [a d c].
+            repeat split; simpl; destruct a as [[|]|]; auto.
+          + unfold M.KeysSubset; apply getDefs_substeps.
+          + unfold M.KeysSubset; apply getCalls_substeps; auto.
+      Qed.
+
+      Lemma multistepMapOne:
+        forall o u l,
+          o = initRegs (getRegInits imp) ->
+          Multistep imp o u l ->
+          exists uSpec ll,
+            thetaR u uSpec /\
+            equivalentLabelSeq (liftToMap1 p) l ll /\
+            Multistep spec (initRegs (getRegInits spec)) uSpec ll.
+      Proof.
+        induction 2; simpl; intros; repeat subst.
+
+        - do 2 eexists; repeat split.
+          + instantiate (1:= initRegs (getRegInits spec)); auto.
+          + instantiate (1:= nil); constructor.
+          + constructor; auto.
+
+        - specialize (IHMultistep eq_refl).
+          destruct IHMultistep as [puSpec [pll ?]]; dest.
+          apply stepMapOne with (oSpec:= puSpec) in HStep; auto;
+            [|eexists; constructor; eauto].
+          destruct HStep as [uSpec [ul ?]]; dest.
+
+          eexists (M.union uSpec puSpec), (ul :: pll).
+          repeat split; auto.
+          + constructor; auto.
+          + constructor; auto.
+      Qed.
+
+      Theorem decompositionOneR:
+        traceRefines (liftToMap1 p) imp spec.
+      Proof.
+        unfold traceRefines; intros.
+        inv H.
+        apply multistepMapOne in HMultistepBeh; auto.
+        destruct HMultistepBeh as [uSpec [ll ?]]; dest.
+        exists uSpec, ll.
+        split; auto.
+        constructor; auto.
+      Qed.
+      
+    End EtaRel.
+
+  End DecompositionOne.
+
+End GivenLabelMap.
+
+Hint Unfold theta etaRState thetaR: MethDefs.
+
+Section DecompositionInv.
+  Variable m: Modules.
+  Variable P: RegsT -> Prop.
+  Hypothesis HinitP: P (initRegs (getRegInits m)).
+
+  Hypothesis HruleP:
+    forall o u rule cs,
+      P o ->
+      Substep m o u (Rle (Some rule)) cs ->
+      P (M.union u o).
+
+  Hypothesis HmethP:
+    forall o u meth cs,
+      P o ->
+      Substep m o u (Meth (Some meth)) cs ->
+      P (M.union u o).
+
+  Lemma substep_P:
+    forall o u ul cs,
+      P o ->
+      Substep m o u ul cs ->
+      P (M.union u o).
   Proof.
-    clear.
-    dependent induction ss; intros; simpl in *.
-    - unfold M.Disj; unfold not; intros.
-      right; intros.
-      apply M.F.P.F.empty_in_iff in H0; intuition.
-    - dependent destruction H.
-      specialize (IHss _ H).
-      destruct a, b; simpl in *.
-      unfold addLabelLeft, mergeLabel, getSLabel; simpl in *.
-      destruct unitAnnot0, unitAnnot; try apply M.Disj_empty_1;
-        try destruct o0; try destruct a; try apply M.Disj_empty_1.
-      case_eq (foldSSLabel ss); intros; simpl.
-      rewrite M.union_empty_L.
-      rewrite H1 in *; simpl in *.
-      assert (sth: forall s', In s' ss ->
-                              canCombine {| substep := substep0 |} s') by
-          (intros; specialize (H0 s'); intuition); clear - sth H1.
-      assert (sth3: defs = Semantics.defs (foldSSLabel ss)) by (rewrite H1; reflexivity).
-      rewrite sth3.
-      eapply defsDisjSs'; eauto.
-      case_eq (foldSSLabel ss); intros; simpl.
-      destruct o1.
-      + destruct a.
-        rewrite H1 in *; simpl in *.
-        assert (sth3: defs = Semantics.defs (foldSSLabel ss)) by (rewrite H1; reflexivity).
-        assert (sth2: M.union (M.add attrName0 attrType0 (M.empty _)) defs =
-                      Semantics.defs (foldSSLabel ({| substep := substep |} :: ss))) by
-            (simpl;
-             unfold addLabelLeft, mergeLabel, getSLabel, getLabel;
-             destruct (foldSSLabel ss); simpl in *; subst; reflexivity).
-        rewrite sth2.
-        eapply defsDisjSs'; eauto.
-      + rewrite M.union_empty_L.
-        rewrite H1 in *; simpl in *.
-        assert (sth: forall s', In s' ss ->
-                                canCombine {| substep := substep0 |} s') by
-            (intros; specialize (H0 s'); intuition); clear - sth H1.
-        assert (sth3: defs = Semantics.defs (foldSSLabel ss)) by (rewrite H1; reflexivity).
-        rewrite sth3.
-        eapply defsDisjSs'; eauto.
+    intros; destruct ul as [[r|]|[dm|]].
+    - eapply HruleP; eauto.
+    - inv H0; mred.
+    - eapply HmethP; eauto.
+    - inv H0; mred.
   Qed.
 
-  Lemma callsDisjSs' m o u a cms (sr: Substep m o u a cms): forall ss,
-      (forall s', In s' ss -> canCombine {| substep := sr|} s') ->
-      M.Disj cms (calls (foldSSLabel ss)).
-  Proof.    
-    clear.
-    dependent induction ss; intros.
-    - apply M.Disj_empty_2.
-    - assert (sth: forall s', In s' ss ->
-                              canCombine {| substep := sr |} s') by
-          (intros; specialize (H s'); intuition).
-      specialize (IHss sth); clear sth.
-      assert (sth2: canCombine {| substep := sr |} a0) by (specialize (H a0); intuition).
-      clear H; unfold canCombine in *.
-      dest.
-      clear H x H0 H1; simpl in *.
-      destruct a0.
-      unfold addLabelLeft, mergeLabel, getSLabel, getLabel; simpl in *.
-      destruct (foldSSLabel ss); simpl in *.
-      apply M.Disj_union; intuition.
-  Qed.
-  
-  Lemma callsDisjSs m o (ss: list (SubstepRec m o)):
-    forall b,
-      substepsComb (b :: ss) ->
-      M.Disj (calls (getSLabel b)) (calls (foldSSLabel ss)).
+  Hypothesis HcanCombine:
+    forall o u1 u2 ul1 ul2 cs1 cs2,
+      Substep m o u1 ul1 cs1 ->
+      Substep m o u2 ul2 cs2 ->
+      CanCombineUL u1 u2 (getLabel ul1 cs1) (getLabel ul2 cs2) ->
+      u1 = M.empty _ \/ u2 = M.empty _.
+
+  Lemma substeps_updates:
+    forall o (s: SubstepRec m o)
+           (ss: Substeps m o),
+      (forall s' : SubstepRec m o, In s' ss -> canCombine s s') ->
+      foldSSUpds ss = M.empty _ \/ upd s = M.empty _.
   Proof.
-    clear.
-    intros.
-    destruct b; simpl in *.
-    unfold addLabelLeft, mergeLabel, getSLabel; simpl in *.
-    case_eq (foldSSLabel ss); intros; simpl in *.
-    assert (sth: Semantics.calls (foldSSLabel ss) = calls) by (rewrite H0; reflexivity).
-    rewrite <- sth.
-    dependent destruction H.
-    eapply callsDisjSs'; eauto.
+    induction ss; simpl; intros; [auto|].
+    assert (forall s' : SubstepRec m o, In s' ss -> canCombine s s').
+    { intros; apply H; auto. }
+    specialize (IHss H0); clear H0.
+    destruct IHss; auto.
+    rewrite H0; mred.
+    specialize (H a (or_introl eq_refl)).
+    apply or_comm.
+    destruct s, a; simpl in *.
+    eapply HcanCombine; eauto.
+    eapply canCombine_CanCombineUL; eauto.
   Qed.
-  
-  Theorem xformLabelFoldCommute o reachO ss:
-    substepsComb ss ->
-    xformLabel o (foldSSLabel (o := o) ss) = foldSSLabel (map (@xformSubstepRec _ reachO ) ss).
+
+  Lemma substeps_P:
+    forall o,
+      P o ->
+      forall (ss: Substeps m o),
+        substepsComb ss ->
+        P (M.union (foldSSUpds ss) o).
   Proof.
-    induction ss; simpl in *; try rewrite liftToMap1Empty; intros.
-    - reflexivity.
-    - pose proof H as sth.
-      dependent destruction H.
-      specialize (IHss H).
-      unfold addLabelLeft in *.
-      rewrite xformLabelAddLabelCommute.
-      f_equal; intuition.
-      apply xformLabelGetSLabelCommute.
-      apply defsDisjSs; intuition.
-      apply callsDisjSs; intuition.
+    induction 2; simpl; intros; [mred|].
+    apply substeps_updates in H1; destruct H1; rewrite H1.
+    - mred.
+      destruct s; simpl in *.
+      eapply substep_P; eauto.
+    - mred.
   Qed.
 
-  Variable impEquiv: ModEquiv type typeUT imp.
-
-  Theorem xformLabelHide o reachO:
-    forall(ss: Substeps imp o) (ssGd: wellHidden imp (hide (foldSSLabel ss))),
-      substepsComb ss ->
-      hide (foldSSLabel (map (@xformSubstepRec _ reachO) ss)) =
-      xformLabel o (hide (foldSSLabel ss)).
+  Lemma multistep_P:
+    forall init n ll,
+      init = initRegs (getRegInits m) ->
+      Multistep m init n ll ->
+      P n.
   Proof.
-    intros.
-    rewrite xformLabelHideCommute.
-    f_equal.
-    apply eq_sym; apply xformLabelFoldCommute; intuition.
-    apply (wellHiddenEq1 (m := imp)).
-    - unfold M.KeysSubset; apply (getDefs_substeps ss).
-    - unfold M.KeysSubset; apply (getCalls_substeps impEquiv ss).
-    - intuition.
+    induction 2; [repeat subst; auto|].
+    specialize (IHMultistep H); subst; clear H0.
+    inv HStep; clear HWellHidden.
+    apply substeps_P; auto.
   Qed.
 
-  Lemma unionCommute' o reachO a state:
-    M.union (upd (@xformSubstepRec o reachO a)) (theta state) =
-    theta (M.union (upd a) state).
+  Lemma decompositionInv:
+    forall o,
+      reachable o m ->
+      P o.
   Proof.
-    destruct a; simpl in *.
-    destruct (substepMap reachO substep).
-    destruct a; simpl in *.
-    intuition.
+    intros; inv H; inv H0.
+    eapply multistep_P; eauto.
   Qed.
-
-  Lemma unionCommute o reachO ss:
-    forall state,
-      M.union (foldSSUpds (map (@xformSubstepRec o reachO) ss)) (theta state) =
-      theta (M.union (foldSSUpds ss) state).
-  Proof.
-    induction ss; intros; simpl in *.
-    - repeat rewrite M.union_empty_L; reflexivity.
-    - rewrite <- M.union_assoc.
-      rewrite <- M.union_assoc.
-      rewrite unionCommute'.
-      apply (IHss (M.union (upd a) state)).
-  Qed.
-
-  Theorem stepMap o (reachO: reachable o imp) u l (s: Step imp o u l):
-    exists uSpec,
-      Step spec (theta o) uSpec (xformLabel o l) /\
-      M.union uSpec (theta o) = theta (M.union u o).
-  Proof.
-    destruct s as [ss ssGd].
-    exists (foldSSUpds (map (@xformSubstepRec _ reachO) ss)).
-    pose proof (wellHiddenSpec o HWellHidden) as sth.
-    pose proof (StepIntro (substepsSpecComb reachO ssGd)) as final.
-    rewrite xformLabelHide in *.
-    specialize (final sth); clear sth.
-    constructor.
-    - intuition.
-    - apply unionCommute; intuition.
-    - intuition.
-    - intuition.
-  Qed.
-
-  Lemma rleEmpty m o u cs:
-    Substep m o u (Rle None) cs -> u = M.empty _ /\ cs = M.empty _.
-  Proof.
-    clear;
-    intros.
-    inversion H; intuition.
-  Qed.
-
-  Lemma methEmpty m o u cs:
-    Substep m o u (Meth None) cs -> u = M.empty _ /\ cs = M.empty _.
-  Proof.
-    clear;
-    intros.
-    inversion H; intuition.
-  Qed.
-
-  Theorem decomposition':
-    forall s sig, Behavior imp s sig ->
-                  exists sigSpec, Behavior spec (theta s) sigSpec /\
-                                  equivalentLabelSeq (liftToMap1 p) sig sigSpec.
-  Proof.
-    intros.
-    dependent induction H.
-    dependent induction HMultistepBeh; subst.
-    - exists nil; rewrite thetaInit; repeat constructor.
-    - specialize (IHHMultistepBeh specRegsCanCombine substepMethMap substepRuleMap
-                                  callSubset defSubset thetaInit eq_refl).
-      clear defSubset0 callSubset0 thetaInit0
-            substepRuleMap0 substepMethMap0 specRegsCanCombine0.
-      assert(reachO: reachable n imp) by (eexists; econstructor; eauto).
-      pose proof (stepMap reachO HStep) as [uSpec [stepSpec upd]].
-      destruct IHHMultistepBeh as [sigSpec [behSpec eqv]].
-      inversion behSpec; subst.
-      pose proof (BehaviorIntro (Multi HMultistepBeh0 stepSpec)) as sth.
-      rewrite upd in sth.
-      exists (xformLabel n l :: sigSpec).
-      constructor.
-      + intuition.
-      + constructor.
-        * unfold equivalentLabel, xformLabel; simpl.
-          destruct l; destruct annot; simpl; intuition.
-          destruct o; simpl; intuition.
-        * intuition.
-  Qed.
-
-  Theorem decomposition:
-    traceRefines (liftToMap1 p) imp spec.
-  Proof.
-    unfold traceRefines; intros.
-    pose proof (decomposition' H) as [sigSpec beh].
-    exists (theta s1); exists sigSpec.
-    intuition.
-  Qed.
-End Decomposition.
-
-Section NoDefs.
-  Variable imp spec: Modules.
-  Variable theta: RegsT -> RegsT.
-  Variable ruleMap: RegsT -> string -> option string.
-  Variable p: string -> (sigT SignT) -> option (sigT SignT).
-  Variable thetaInit: theta (initRegs (getRegInits imp)) = initRegs (getRegInits spec).
-  Variable defSubset: forall f, In f (getDefs spec) -> In f (getDefs imp).
-  Variable callSubset: forall f, In f (getCalls spec) -> In f (getCalls imp).
-
-  Variable substepRuleMap:
-    forall oImp uImp rule csImp,
-      reachable oImp imp ->
-      Substep imp oImp uImp (Rle (Some rule)) csImp ->
-      { uSpec |
-        Substep spec (theta oImp) uSpec (Rle (ruleMap oImp rule)) (liftToMap1 p csImp) /\
-        forall o, M.union uSpec (theta o) = theta (M.union uImp o) }.
-
-  Variable impEquiv: ModEquiv type typeUT imp.
-
-  Hypotheses HnoDefsImp: getDefsBodies imp = nil.
-  
-  Corollary decomposition_nodefs:
-    traceRefines (liftToMap1 p) imp spec.
-  Proof.
-    eapply decomposition with (theta:= theta)
-                                (ruleMap:= ruleMap)
-                                (substepRuleMap:= substepRuleMap); eauto.
-    intros; exfalso; destruct H.
-    - destruct s1 as [u ul calls Hss]; simpl in *; subst.
-      inv Hss; rewrite HnoDefsImp in HIn; inv HIn.
-    - destruct s2 as [u ul calls Hss]; simpl in *; subst.
-      inv Hss; rewrite HnoDefsImp in HIn; inv HIn.
-
-      Grab Existential Variables.
-      { intros; exfalso; inv H0.
-        rewrite HnoDefsImp in HIn; inv HIn.
-      }
-  Qed.
-
-End NoDefs.
+      
+End DecompositionInv.
 
